Added considerable doc-comments

src/Untyped/Beta.v
@@ -1,20 +1,63 @@
-Add LoadPath "./src/Untyped/".
+(** * Beta Reduction and Reduction Schemes
 
-Module src.
-Module Untyped.
-Module Beta.
+This is the bread-and-butter of lambda calculus. We apply
+an argument to a function, that's the goal. How? We have
+lambda abstractions introduce one bound variable, a "named
+parameter" if you will: [λ x . M] introduces a single
+variable [x].
+
+Application is intended to _apply_ an expression to the
+function. How? By _substituting_ for that bound variable,
+the second expression. That is to say, [(λ x . M) N]
+intuitively should "evaluate" to [[x:=N]M].
+
+This "evaluation procedure" is called _Beta Reduction_.
+We can implement it as a function...or we can think of it
+as a process [(λ x . M) N -> [x:=N]M]. If we think of it
+as a process, then we can form a _relation_...more like
+[(λ x . M) N > [x:=N]M] which is either [True] or [False].
+So, in this light, Beta reduction is a [Prop].
+
+But how do we start reducing expressions? In something 
+like [(λ x . I I I M) N], where [I] is the [I] combinator,
+we could start reducing the body [I I I M -> I I M -> I M]
+and so on. Or we could substitute [x:=N] to the body, then
+start reducing. Does it matter? Will it produce the same
+results? What if we had [(λ x . I I I M) (I I I N)]?
+Can we start reducing [(I I I N) -> I I N -> I N -> N]?
+
+The answers here are quite obviously "It doesn't matter,
+they produce the same result". But that's only because we
+used the identity combinator. What if we used [S] or [K]?
+It's no longer immediately obvious whether we must be
+careful where to start beta reducing, or whether we may
+be sloppy.
+
+What about handling paradoxical combinators like 
+[Combinator.Omega] (Ω = ωω, where ω = λx. x x)? If we
+tried naively to evaluate this, we'd get a nonterminating
+program. That's bad. Really bad. So bad, we want to
+desperately avoid this!
+
+We'll first introduce beta reduction, then we'll discuss
+various "reduction schemes" determining how to evaluate
+expressions and reduce them.
+*)
 Require Import String.
 Require Import Coq.Arith.EqNat.
-Require Import Coq.Relations.Relation_Operators.
+Require Import Relation_Operators.
 
+Require Import TractLib.
 Require Import Syntax.
 Require Import Substitute.
 
-(**
-  Beta reduction amounts to taking a term of the form
-  [(lambda x . b) t] and producing [[x:=t]b]. If the term given
-  is not of this form, then return the term. In this manner, it
-  acts like the identity.
+Module Export Beta.
+(** ** Beta Reduction
+
+Beta reduction amounts to taking a term of the form
+[(lambda x . b) t] and producing [[x:=t]b]. If the term
+given is not of this form, then return the term. In 
+this manner, it acts like the identity.
 *)
 
 Fixpoint Beta (t:Term) : Term :=
@@ -27,6 +70,11 @@ Fixpoint Beta (t:Term) : Term :=
   | _ => t
   end.
 
+(**
+We see that, for any term [t], we have 
+[Combinator.I t -> t]. This merits thinking of [Combinator.I]
+as the "identity function".
+*)
 Example i_combinator_is_identity :
   forall (t : Term),
   Beta (App Combinator.I t) = t.
@@ -36,8 +84,11 @@ Proof.
   unfold Beta; unfold Combinator.I; unfold subst; apply eq_id.
 Qed.
 
-(** Definition. A term is in Beta Normal Form iff it doesn't have any
-    subterms of the form [App (lambda x. body) R]. *)
+(**
+Definition (Barendregt 2.1.34). 
+A term is in Beta Normal Form iff it doesn't have any
+subterms of the form [App (lambda x. body) R].
+*)
 Fixpoint BetaNF (M:Term) : Prop :=
   match M with
   | BVar _ => True
@@ -47,10 +98,12 @@ Fixpoint BetaNF (M:Term) : Prop :=
   | App M' N => (BetaNF M')/\(BetaNF N)
   end.
 
-(** What expression wouldn't be in Beta normal form? One that would never
-    terminate. For example, the [Combinator.Omega] evaluates to itself after
-    beta reduction, so if we tried repeatedly beta reducing...we'll end up in
-    an infinite loop. Which may be bad.
+(**
+What expression wouldn't be in Beta normal form? One that
+would never terminate. For example, the [Combinator.Omega]
+evaluates to itself after beta reduction, so if we tried 
+repeatedly beta reducing...we'll end up in an infinite 
+loop. Which may be bad.
 *)
 Example Omega_combinator_isnt_beta_nf :
   ~(BetaNF Combinator.Omega).
@@ -64,7 +117,21 @@ Proof.
   simpl; tauto. (* And it's obvious. *)
 Qed.
 
+(**
+Even unfolding the definition of [Combinator.Omega] once with
+beta reduction produces [Combinator.Omega]!
+*)
+Example Omega_combinator_evaluates_to_itself :
+  Beta Combinator.Omega = Combinator.Omega.
+Proof.
+  unfold Combinator.Omega; unfold Combinator.omega.
+  unfold Beta. unfold subst. rewrite eq_id.
+  reflexivity.
+Qed.
+
+
 (** * Values
+
 
 We would like to think of Beta reduction as one step in an abstract
 "processor". A value would be where the Beta reduction would stop after
@@ -112,9 +179,13 @@ Inductive step : Term -> Term -> Prop :=
 where "t1 '==>' t2" := (step t1 t2).
 Hint Constructors step.
 
-Notation multistep := (clos_refl_trans step).
+
+Notation multistep := (multi step).
 Notation "t1 '==>*' t2" := (multistep t1 t2) (at level 40).
 
+Example Omega_steps_to_itself:
+  Combinator.Omega ==>* Combinator.Omega.
+Proof.
+  apply multi_refl.
+Qed.
 End Beta.
-End Untyped.
-End src.
