src/Untyped/Syntax.v
@@ -1,39 +1,33 @@
-(* If you run into problems, try adding the following line:
-
-Add LoadPath "~/src/tractatus/src/Untyped/".
-
-...modify it to where the folder is, accordingly. *)
-
-Module Export src.
-Module Export Untyped.
 Module Export Syntax.
 Require Import String.
 Require Import List.
 Require Export Arith.
 Require Import Coq.Arith.EqNat.
 Require Import Coq.Arith.Compare_dec.
+Require Import TractLib.
 
-(** Helper lemmas, which should be refactored into a different module.
+(** * Introduction: Lambda Calculus
 
-Principle of explosion: from a contradiction, we can prove anything. 
+Lambda calculus is the smallest complete programming language in the world.
+We can perform, really, two operations: (1) form functions, (2) apply 
+arguments to functions.
+
+We'll construct the basic abstract syntax tree for untyped lambda calculus,
+then develop other mechanisms in other files.
+
+The basic concept for untyped lambda calculus is the "expression" or "term",
+which can be an "identifier", a "function", or an "application". Lets 
+first develop the framework for "names" (or "identifiers").
 *)
-Theorem ex_falso_quodlibet : forall (P:Prop),
-  False -> P.
-Proof.
-  intros P contra.
-  inversion contra.
-Qed.
-
-Lemma list_membership :
-  forall (A:Type) (x:A) (l1 l2:list A),
-  (In x l1)\/(In x l2) <-> In x (l1 ++ l2).
-Proof. intuition. Qed.
-(* End of Helper Lemmas *)
 
 (** * Identifiers and Variables
 
-We treat variables and identifiers on unequal footing, depending on if they are
-free or bound.
+For lambda calculus, identifiers are used to...identify...variables. And
+variables are only used as parameters in functions. They do not store
+values, as they would in modern programming languages.
+
+We treat both variables, and identifiers, on unequal footing...in the sense
+that we specify if they are free or bound.
 *)
 
 Module Export Identifier.
@@ -60,9 +54,9 @@ Lemma eq_id : forall (T:Type) x (p q:T),
 Proof.
   intros.
   destruct (eq_id_dec x x).
-  (* Case: [x=x] *)
+  Case "x=x".
     try reflexivity.
-  (* Case: [x<>x] (impossible) *)
+  Case "x<>x". (* impossible *)
     apply ex_falso_quodlibet; auto.
 Qed.
 
@@ -71,10 +65,9 @@ Lemma neq_id : forall (T:Type) x y (p q:T), x <> y ->
 Proof.
   intros.
   destruct (eq_id_dec x y).
-  (* Case x = y (impossible) *)
+  Case "x=y". (* impossible *)
     subst. apply ex_falso_quodlibet; apply H; reflexivity.
-  (* Case x <> y *)
-    reflexivity.
+  Case "x <> y". reflexivity.
 Qed.
 End Identifier.
 
@@ -88,20 +81,68 @@ Lambda calculus is defined, inductively, by constructing terms. A term may be:
 
 - an application _M N_ for arbitrary terms _M_ and _N_.
 
+
 Observe there are no quantifiers in the theory, since lambda calculus is an
 equational theory. It is not a logical calculus. (But it can encode one!) So
 any quantifiers used are purely in the metalanguage.
 
-How do we represent a term in our metalanguage?
+The grammar for this can be written quite quickly in BNF:
+
+<<
+<term> ::= <variable>
+         | 'λ' <variable> '.' <term>
+         | <term> <term>
+>>
+
+The problem is...How do we represent a term in our metalanguage?
 
 ** De Bruijn Indices
-  We use a modified de Bruijn indices, which for free variables
-  are a string, and for bound variables...it's the usual de Bruijn
-  index.
+
+Suppose all variables are "bound", meaning they first show up in
+a lambda expression defining it. The only way to introduce a variable
+[x] is to write [λ x . M] for some [M]. One trick, credited to
+Niklaus de Bruijn (prenounced "de Browne"), is to use numbers for
+bound variables. This makes it easy to determine if a variable is
+free or bound, and substitution just looks for the proper number.
+
+There's more to this trick, however. The number we give to a bound
+variable is "How 'deeply nested' the variable is, from its declaration."
+Lets give a couple of examples to illustrate what this means.
+
+- Consider [λx. λy. x].
+  - Since we have only 1 bound variable [x] in the body of the
+    our second lambda expression, we have to replace it with a 
+    number. And since it's bound to the _first_ lambda expression,
+    one layer above where it's used (that's the important bit), we
+    replace it with [1]. The de Bruijn indices then kill off the
+    variables in the declaration, since they're now represented by
+    numbers, giving us [λλ1].
+  - If we had instead [λx. λy. y], then it would be [λλ0] since [y]
+    is used in the body of the lambda where it is declared.
+- Consider [λx. λy. λz. x z (y z)].
+  - Starting with the innermost lambda abstraction, we see [z] is used
+    in the body of the lambda declaring it. We can replace it with
+    [λx. λy. λ(x 0 (y 0))].
+  - Next, we have the [y] variable to replace. Since it is declared one
+    abstraction _above_ the body of the lambda where it is used, we
+    replace it with [1], giving us [λx. λλ. (x 0 (1 0))].
+  - Lastly, we have [x], which is declared 2 layers above the body
+    where it is used. So we replace it with [2]: [λλλ. (2 0 (1 0))].
+
+
+Our discussion so far has been concerning variables first declared
+in a lambda expression, i.e., "bound" variables. What if the user
+puts in variables _not_ "bound" to a lambda expression? For example,
+[λ x . z], what happens to [z] ("free variables")?
+
+We use a modified de Bruijn indices, which for free variables
+are a string, and for bound variables...it's the usual de Bruijn
+index.
   
-  The reason this is preferable, we didn't want [lambda [x] y] to
-  match [lambda [x] z], which the usual de Bruijn indices would not
-  handle.
+The reason this is preferable, we didn't want [lambda [x] y] to
+match [lambda [x] z], which the usual de Bruijn indices would not
+handle...at least, not without some _global_ notion of which variables 
+have been "used up" and which ones are "fresh".
 *)
 Module Export DeBruijn.
 
@@ -113,6 +154,39 @@ Inductive Term : Type :=
 Hint Constructors Term.
 End DeBruijn.
 
+(**
+This crops up later, but it's useful to know if a given term is an abstraction
+("function") or not.
+*)
+Definition is_abs (t:Term) : Prop :=
+  match t with
+  | Lam _ => True
+  | _ => False
+  end.
+
+(**
+For the sake of completeness, we'll also provide predicates for if a term is a
+variable, an application, etc.
+*)
+Definition is_var (t:Term) : Prop :=
+  match t with
+  | FVar _ => True
+  | BVar _ => True
+  | _ => False
+  end.
+
+Definition is_free_var (t:Term) : Prop :=
+  match t with
+  | FVar _ => True
+  | _ => False
+  end.
+
+Definition is_app (t:Term) : Prop :=
+  match t with
+  | App _ _ => True
+  | _ => False
+  end.
+
 (** **** Exercise
 
 Show if [FVar s = FVar s0], then [s = s0].
@@ -121,15 +195,18 @@ Lemma FVar_eq :
   forall (s s0:string),
   (FVar s0) = (FVar s) <-> s=s0.
 Proof.
+(* Left for the reader ;) *)
+(* begin hide *)
   intuition.
-  (* -> s=s0 *)
-    inversion H; reflexivity.
-  (* <- (FVar s0) = (FVar s) *)
-    rewrite H; reflexivity.
+  Case "s=s0". inversion H; reflexivity.
+  Case "(FVar s0) = (FVar s)". rewrite H; reflexivity.
+(* end hide *)
 Qed.
 
-(** The free variables in a term is just a list of all the free variables
-    appearing in it. This is just Barendregt, definition 2.1.7.i.
+(**
+The free variables in a term is just a list of all the free variables
+appearing in it. We have a function [FV] to obtain this list!
+This is just Barendregt, definition 2.1.7.i.
 *)
 Fixpoint FV (t : Term) : list Term :=
   match t with
@@ -139,19 +216,34 @@ Fixpoint FV (t : Term) : list Term :=
   | App t' t'' => app (FV t') (FV t'')
   end.
 
-(** Applying one term to another preserves the free variables in
-    the representation we have chosen. Why? Because we explicitly treat
-    free variables _differently_ than bound ones. Application could
-    consume bound variables, but not free variables.
+(**
+*** Exercise
+Show that [forall (v t:Term), In v (FV t) -> is_free_var v].
+*)
+
+(**
+*** Helper Functions
+
+Applying one term to another preserves the free variables in
+the representation we have chosen. Why? Because we explicitly treat
+free variables _differently_ than bound ones. Application could
+consume bound variables, but not free variables.
+
+_Remark_. 
+Note that "functorial" is used loosely. Although, I suppose one
+could make the argument it's a "functor" from the [tree] underlying
+the Abstract Syntax Tree, to the [list] of free variables, preserving
+concatenation. But it's not an honest, mathematical functor!
 *)
 
 Proposition app_FV_functorial :
   forall (M1 M2:Term),
-  FV (App M1 M2) = (FV M1) ++ (FV M2).
+  FV (App M1 M2) = app (FV M1) (FV M2).
 Proof. intuition. Qed.
 
-(** We have a property determining if an [Id] is a free variable in a term or not. 
-    (Should this be an [Inductive] type instead? I'm uncertain)
+(**
+We have a property determining if an [Id] is a free variable in a term or not. 
+(Should this be an [Inductive] type instead? I'm uncertain)
 *)
 Definition Id_in_FV (x:Id) (t:Term) : Prop :=
   match x with
@@ -159,6 +251,13 @@ Definition Id_in_FV (x:Id) (t:Term) : Prop :=
   | _ => False
   end.
 
+(**
+Let [x] is a free variable. 
+
+The identifier [i] is in [FV(x)] 
+if and only if
+the string representation of [x] _is_ the string representation of [i].
+*) 
 Lemma trivial_FV_in_FV :
   forall (s s0:string),
   Id_in_FV (FId s0) (FVar s) <-> s=s0.
@@ -170,6 +269,9 @@ Proof.
   rewrite H. unfold Id_in_FV; unfold FV; compute; auto.
 Qed.
 
+(**
+The converse is also true.
+*)
 Lemma trivial_FV_notin_FV :
   forall (s s0:string),
   s<>s0 <-> ~(Id_in_FV (FId s0) (FVar s)).
@@ -181,6 +283,10 @@ Proof.
   apply trivial_FV_in_FV in H0; contradiction.
 Qed.
 
+(**
+And it follows that if [x] is a bound variable, then no free variable could
+ever hope to be in [FV(x)]...because [FV(x)] is [nil].
+*)
 Corollary trivial_FV_notin_BV :
   forall (s:string) (n:nat),
   ~(Id_in_FV (FId s) (BVar n)).
@@ -195,6 +301,13 @@ Proof.
   unfold Id_in_FV; rewrite app_FV_functorial; apply list_membership.
 Qed.
 
+(** * A Prettier Syntax
+
+We allow a user to write a more palatable version of lambda calculus, which we then
+transform into our abstract syntax tree representation.
+
+*)
+
 Module PrettyTerm.
 
 Inductive pterm : Type :=
@@ -206,6 +319,7 @@ Hint Constructors pterm.
 End PrettyTerm.
 
 Notation "` x" := (PrettyTerm.Var x) (at level 20).
+Notation "x '~>' M" :=  (PrettyTerm.Lam x M) (at level 30).
 Notation "'lambda' [ x , .. , y ] M" := (PrettyTerm.Lam x .. (PrettyTerm.Lam y M) .. ) (at level 30).
 Infix "@" := PrettyTerm.App (at level 25, left associativity).
 
@@ -229,12 +343,12 @@ Proof. reflexivity. Qed.
 
 (** ** Syntactic Sugar: [PrettyTerm] to [Term]
 
-  We basically want to write lambda expressions using the [PrettyTerm],
-  but we want it to be converted to [DeBruijn.Term] using the "obvious"
-  de Bruijn indexing notation, with the exception that free variables are
-  kept as strings. (This is to prevent contradictory results --- if we
-  used de Bruijn indexing convention on free variables, we'd have results like
-  [lambda [x] `"y" = lambda [x] `"z"], which we don't want.)
+We basically want to write lambda expressions using the [PrettyTerm],
+but we want it to be converted to [DeBruijn.Term] using the "obvious"
+de Bruijn indexing notation, with the exception that free variables are
+kept as strings. (This is to prevent contradictory results --- if we
+used de Bruijn indexing convention on free variables, we'd have results 
+like [lambda [x] `"y" = lambda [x] `"z"], which we don't want.)
 *)
 
 Fixpoint lookup (s: string) (ls: list (string * nat)) : option nat :=
@@ -243,10 +357,11 @@ Fixpoint lookup (s: string) (ls: list (string * nat)) : option nat :=
   | (x, n) :: t => if string_dec x s then Some n else lookup s t
   end.
 
-(** We need to keep track of the bound variables, without adding duplicates.
-    The helper function [hide] takes care of this for us.
-    If the variable [s] is not in the lookup, add it associated
-    to [0] (zero). This is the usual de Bruijn indexing scheme.
+(**
+We need to keep track of the bound variables, without adding duplicates.
+The helper function [hide] takes care of this for us.
+If the variable [s] is not in the lookup, add it associated
+to [0] (zero). This is the usual de Bruijn indexing scheme.
 *)
 
 Fixpoint hide (s: string) (ls: list (string * nat)) : list (string * nat) :=
@@ -255,6 +370,11 @@ Fixpoint hide (s: string) (ls: list (string * nat)) : list (string * nat) :=
   | (x, n) :: t => if string_dec x s then (x, 0) :: hide s t else (x, n + 1) :: hide s t
   end.
 
+(**
+We take a pretty term and a list of bindings, and recursively
+translate to the internal abstract syntax tree representation for the
+expression.
+*)
 Fixpoint dename' (t: PrettyTerm.pterm) (binds: list (string * nat)) : Term :=
   match t with
   | PrettyTerm.Var s => match lookup s binds with
@@ -270,17 +390,17 @@ Definition dename (t : PrettyTerm.pterm) : Term :=
 
 Coercion dename : PrettyTerm.pterm >-> Term.
 
-(** These are basically a couple of proofs with all the
-    scratchwork, and proof states, noted for the sake of
-    pedagogy/pedantic-mania.
-*)
+(**
+These are basically a couple of proofs with all the
+scratchwork, and proof states, noted for the sake of
+pedagogy/pedantic-mania.
 
-(** This lemma basically says that free variables that aren't
-    equal won't produce equal terms.
+This lemma basically says that free variables that aren't
+equal won't produce equal terms.
 
-    The naive de Bruijn indexing scheme can't prove this, and it's
-    fairly important that [lambda [x] y <> lambda [x] z] whenever [y <> z].
-    (And [<>] is read as "not equals".)
+The naive de Bruijn indexing scheme can't prove this, and it's
+fairly important that [lambda [x] y <> lambda [x] z] whenever [y <> z].
+(And [<>] is read as "not equals".)
 *)
 Lemma free_variables_dont_match_lam :
   forall (x y z : string),
@@ -288,10 +408,9 @@ Lemma free_variables_dont_match_lam :
   ((lambda [x] `"y") <> (lambda [x] `"z")).
 Proof.
   (* Introduce the variables, and the hypothesis
-     [H : y <> z] *)
-  intros.
-  (* [intuition] sets us up for a proof by contradiction.
-     That is, it assumes [H0 : lambda [x] `y = lambda [x] `z],
+     [H : y <> z]. Here, [intuition] sets us up for a proof 
+     by contradiction. That is, it assumes 
+     [H0 : lambda [x] `y = lambda [x] `z],
      rewrites the hypothesis as [H : y = z -> False], and
      the goal is now [False] *)
   intuition.
@@ -299,9 +418,10 @@ Proof.
   inversion H0.
 Qed.
 
-(** It is a necessary condition for the free variables of
-    term [t] to be equal to the free variables of term [t'] for
-    [t = t']. And we can prove it!
+(**
+It is a necessary condition for the free variables of
+term [t] to be equal to the free variables of term [t'] for
+[t = t']. And we can prove it!
 *)
 Theorem free_var_match_necessary_cond_term_eq :
   forall (t t' : Term),
@@ -316,27 +436,48 @@ Qed.
 
 (** Definitions are taken from Barendregt's _Lambda Calculus_. *)
 
-(** The SKI combinators. Barendregt 2.1.25. We also have included the Omega combinator. *)
+(** ** Combinators
+
+**** Definition
+
+A _Combinator_ is a term with no free variables, only bound variables.
+
+**** SKI Combinators and Friends
+
+The SKI combinators. Barendregt 2.1.25.
+
+There is a folklore theorem stating any combinator may be written in
+terms of SKI combinators...which explains their importance.
+
+We also have included the Omega combinator, which paradoxically evaluates to itself.
+*)
 
 Module Combinator.
 
-(** We have the classic [S], [K], and [I] combinators, which famously generate any
-    closed term.
+(**
+We have the classic [S], [K], and [I] combinators, which famously generate any
+closed term. Recall:
+
+- [I = λx. x] is the identity combinator,
+
+- [K = λx. λy. y] is the constant combinator
+
+- [S = λx. λy. λz. x z (y z)] a generalized application.
 *)
 Definition I : Term := Lam (BVar 0).
-Hint Unfold I.
-Definition K : Term := Lam (Lam (BVar 1)).
-Hint Unfold K.
-Definition S : Term := Lam (Lam (Lam (App (App (BVar 2) (BVar 0)) (App (BVar 1) (BVar 0))))).
-Hint Unfold S.
+Definition K : Term := 
+  Lam (Lam (BVar 1)).
+Definition S : Term := (* λx. λy. λz. x z (y z) *)
+  Lam (Lam (Lam (App (App (BVar 2) (BVar 0)) (App (BVar 1) (BVar 0))))).
 
-(** We also have a nonterminating [Omega] combinator, which --- if
-    evaluated --- produces itself.
+
+(**
+We have the application combinator [omega] (ω = λx. x x).
+We also have a nonterminating [Omega] (Ω) combinator, which --- if
+evaluated --- produces itself.
 *)
-Definition omega : Term := App (App S I) I.
-Hint Unfold omega.
+Definition omega : Term := Lam (App (BVar 0) (BVar 0)).
 Definition Omega : Term := App omega omega.
-Hint Unfold Omega.
 
 End Combinator.
 
@@ -344,9 +485,9 @@ Example s_dename_ex1 :
   dename (lambda ["x", "y", "z"] `"x" @ `"z" @ (`"y" @ `"z")) = Combinator.S.
 Proof. simpl; reflexivity. Qed.
 
-(** **** Closed Terms
+(** *** Closed Terms
 
-  A term is "closed" if it has no free variables. (Barendregt, 2.1.7.ii.) 
+A term is "closed" if it has no free variables. (Barendregt, 2.1.7.ii.) 
 *)
 Inductive closed : Term -> Prop :=
   | fvar_closed : forall (s:string), closed (FVar s)
@@ -373,17 +514,24 @@ Proof.
   unfold Combinator.K; auto.
 Qed.
 
-(** **** Subterms
+(** *** Subterms
 
- The collection of subterms of a given term. (Barendregt, 2.1.8.)
+(Barendregt, 2.1.8.) The collection of subterms of a given term. Variables
+have no subterms except themselves: they're as simple as we can get.
+
+A lambda expression has a body, so the expression plus subterms of the body
+produces the subterms for the expression as a whole.
+
+Similarly, application takes two arguments, so their subterms plus the
+expression produces the subterms for the application expression.
 *)
 Fixpoint subterms (t : Term) : list Term :=
-  t::(match t with
-      | FVar _ => nil
-      | BVar _ => nil
-      | Lam t' => (subterms t')
-      | App t' t'' => (subterms t') ++ (subterms t'')
-      end).
+  match t with
+  | FVar _ => t::nil
+  | BVar _ => t::nil
+  | Lam t' => t::(subterms t')
+  | App t' t'' => t::(app (subterms t') (subterms t''))
+  end.
 
 Example i_subterms : 
   subterms Combinator.I = Combinator.I :: (BVar 0) :: nil.
@@ -409,7 +557,13 @@ Example s_subterms :
                  :: nil.
 Proof. reflexivity. Qed.
 
-(** Barendregt 2.1.9. Modified slightly to handle the [n=0] case. *)
+(** **** Iterative Applications
+
+Barendregt 2.1.9. If we write, say, [M^n N], we should understand this means
+[M M M ... M N] where [M] has been repeated [n] times. We have a function for that,
+writing [M^n N = App (iterate n M) N]. Our definitions modifies Barendregt's
+slightly to handle the [n=0] case. 
+*)
 Fixpoint iterate (n : nat) (t : Term) : Term :=
   match n with
   | 0 => Combinator.I
@@ -417,14 +571,16 @@ Fixpoint iterate (n : nat) (t : Term) : Term :=
   | S n' => App t (iterate n' t)
   end.
 
-(** The length of a term is the (number of free variables) + (number of lambdas) 
-    + (number of de Bruijn indices).
+(** **** Term Length
 
-    Don't be fooled by the similarity between [length] and [subterms].
-    It turns out the length of the list of [subterms] is not equal to the
-    [length] of a term. For a counter-example, consider a term like
-    [App t1 t2]. Its subterms would produce [(App t1 t2)::((Subterms t1)++(Subterms t2))].
-    But its length would be [(length t1) + (length t2)].
+The length of a term is the (number of free variables) + (number of lambdas) 
++ (number of de Bruijn indices).
+
+Don't be fooled by the similarity between [length] and [subterms].
+It turns out the length of the list of [subterms] is not equal to the
+[length] of a term. For a counter-example, consider a term like
+[App t1 t2]. Its subterms would produce [(App t1 t2)::((Subterms t1)++(Subterms t2))].
+But its length would be [(length t1) + (length t2)].
 *)
 Fixpoint length (t : Term) : nat :=
   match t with
@@ -445,8 +601,11 @@ Proof. reflexivity. Qed.
 Example s_length :
   length Combinator.S = 7.
 Proof. reflexivity. Qed.
-
-
 End Syntax.
-End Untyped.
-End src.
+
+(** * References
+
+- Barendregt, _The Lambda Calculus, Its Syntax and Semantics_.
+- Stanford Encyclopedia of Philosophy entry, http://plato.stanford.edu/entries/lambda-calculus/
+- Raul Rojas, "A Tutorial Introduction to the Lambda Calculus".
+*)
