src/Untyped/Substitute.v
@@ -1,17 +1,18 @@
-Add LoadPath "./src/Untyped/".
-
 (** printing ==> #<span style="font-family: arial;">&rArr;</span># *)
 (** printing ==>* #<span style="font-family: arial;">&rArr;*</span># *)
+(** * Substitution
 
-(**
 Lambda calculus really shines at substitution. Arguably, its entire
-_raison d'etre_ is to study how to substitute terms into expressions.
-But there's a lot of subtlety here, we don't want to fall into traps.
-*)
+_raison d'être_ is to study how to substitute terms into expressions,
+i.e., apply an argument to a function.
 
-Module Export src.
-Module Export Untyped.
+But there's a lot of subtlety here, we don't want to fall into traps.
+Care must be taken when working with free variables versus
+bound variables.
+*)
 Module Export Substitute.
+
+
 Require Import String.
 Require Import Coq.Arith.EqNat.
 Require Import Coq.Relations.Relation_Operators.
@@ -28,8 +29,12 @@ Definition (Barendregt 2.1.15). The result of substituting
  - [[x:=N] (App M1 M2) = App ([x:=N]M1) ([x:=N]M2)]
 *)
 Reserved Notation "'[' x ':=' s ']' t" (at level 20).
-
-(* Substitute [s] for [x] in term [t]. *)
+(**
+Substitute [s] for [x] in term [t]. There is some subtlety when
+[x] is a bound variable, because we need to keep track of which
+lambda it is "bound" to...this is due to using the de Bruijn
+index convention.
+*)
 Fixpoint subst (x:Id) (s:Term) (t:Term) : Term :=
   match t with
   | FVar x' => if (eq_id_dec (FId x') x) then s else t
@@ -43,8 +48,10 @@ Fixpoint subst (x:Id) (s:Term) (t:Term) : Term :=
 where "'[' x ':=' s ']' t" := (subst x s t).
 
 
-(** Here are a few "helper functions" with [subst] that should be
-    immediately obvious.
+(**
+Here are a few "helper functions" with [subst] that should
+be immediately obvious. Substituting [x:=N] in [x] should
+be [N], obviously.
 *)
 Lemma subst_free_var :
   forall (x:string) (N:Term),
@@ -54,8 +61,62 @@ Proof.
   unfold subst. apply eq_id.
 Qed.
 
-(** Substitution must match the variable being replaced. Otherwise,
-    it acts like the identity. *)
+(**
+We can combine the previous results to get something
+almost nontrivial. Suppose [x<>y], and [x] does not 
+appear in [L]. Then substituting [[y:=L]N] for [x]
+produces [[y:=L]N].
+*)
+Lemma unfold_one_step :
+  forall (x y:string) (L N:Term),
+  x<>y ->
+  ~(Id_in_FV (FId x) L) ->
+  [FId x := [FId y := L]N]FVar x = [FId y:=L]N.
+Proof.
+  intros.
+  unfold subst.
+  apply eq_id.
+Qed.
+
+(**
+A helper lemma unfolding the definition of substitution:
+Substituting [N] for a free variable in [Lam M] amounts 
+to considering the lambda abstraction of substituting 
+[N] for that free variable in [M].
+*)
+Lemma subst_lambda_swap :
+  forall (x:string) (M N:Term),
+  [FId x:=N]Lam M=Lam([FId x:=N]M).
+Proof.
+  intuition.
+Qed.
+
+(**
+Another helper lemma unfolding the definition of
+substitution:
+Substituting [x:=N] in [M1 M2] produces the application
+of substituting [x:=N] in M2 to substituting [x:=N] M1.
+*) 
+Lemma subst_app_functoriality :
+  forall (x:string) (M1 M2 N:Term),
+  [FId x:=N]App M1 M2=App ([FId x:=N]M1) ([FId x:=N]M2).
+Proof.
+  intuition.
+Qed.
+
+(** ** Substitution defaults to the Identity Operation
+
+Consider this general situation [[x:=L]M] but [x] is not
+a free variable in [M]. There's nothing to substitute! So
+we'd expect [[x:=L]M = M], nothing should happen. We'll
+present a theorem saying as much, but first we need a
+couple lemmas to simplify the proof.
+
+First, we have the case of [M] being a free variable
+[y<>x]. Substitution must match the variable being 
+replaced. Otherwise, it acts like the identity. And we
+can prove it!
+*)
 Lemma subst_free_var_denied :
   forall (x y:string) (L:Term),
   x<>y -> ([FId y := L]FVar x)=FVar x.
@@ -68,8 +129,9 @@ Proof.
   reflexivity.
 Qed.
 
-(** Substituting a term for a free variable, again, acts like the identity
-    operation when acting on a bound variable.
+(**
+Capture-free substitution acting on a _bound_ variable,
+by definition, won't change the bound variable.
 *)
 Lemma subst_bvar_denied :
   forall (x:string) (n:nat) (L:Term),
@@ -81,46 +143,16 @@ Proof.
   discriminate. (* by looking at it! *)
 Qed.
 
-Lemma identity_subst :
-  forall (y:string) (L:Term),
-  [FId y := L]FVar y = L.
-Proof.
-  intuition.
-  unfold subst; rewrite eq_id; reflexivity.
-Qed.
+(**
+Generally, substitution acts like the identity operation
+on a term when we try to substitute a term for an
+absent variable.
 
-Lemma unfold_one_step :
-  forall (x y:string) (L N:Term),
-  x<>y ->
-  ~(Id_in_FV (FId x) L) ->
-  [FId x := [FId y := L]N]FVar x = [FId y:=L]N.
-Proof.
-  intros.
-  unfold subst.
-  apply eq_id.
-Qed.
-
-(** Substituting [N] for a free variable in [Lam M] amounts to considering
-    the lambda abstraction of substituting [N] for that free variable in [M].
+If we try to substitute [N] for [s] in [M], but [s] 
+isn't in [M], then nothing happens. The substitution 
+operation should return to us [M].
 *)
-Lemma subst_lambda_swap :
-  forall (x:string) (M N:Term),
-  [FId x:=N]Lam M=Lam([FId x:=N]M).
-Proof.
-  intuition.
-Qed.
-
-Lemma subst_app_functoriality :
-  forall (x:string) (M1 M2 N:Term),
-  [FId x:=N]App M1 M2=App ([FId x:=N]M1) ([FId x:=N]M2).
-Proof.
-  intuition.
-Qed.
-
-(** If we try to substitute [N] for [s] in [M], but [s] isn't in [M], then
-    nothing happens. The substitution operation should return to us [M].
-*)
-Lemma absent_id_doesnt_subst :
+Theorem absent_id_doesnt_subst :
   forall (s:string) (M N:Term),
   ~(Id_in_FV (FId s) M) -> [(FId s):=N]M = M.
 Proof.
@@ -168,7 +200,7 @@ Lemma substitution_lemma_subcase_12 :
 Proof.
   intros.
   rewrite subst_free_var; rewrite subst_free_var_denied.
-  rewrite identity_subst. rewrite absent_id_doesnt_subst. reflexivity.
+  rewrite subst_free_var. rewrite absent_id_doesnt_subst. reflexivity.
   inversion H. assumption. inversion H. auto.
 Qed.
 
@@ -218,9 +250,15 @@ Proof.
   - repeat (rewrite subst_app_functoriality).
     rewrite IHM1; rewrite IHM2; reflexivity. (* Then by inductive hypothesis, it's true. *)
 Qed.
-(** [] *)
 
-(** Barendregt 2.1.17.i *)
+(** ** Substitution in Applications
+
+If we have [M = M'], then we have a variety of ways to substitute
+[N] into this expression. 
+
+(Barendregt 2.1.17.i) If we have [M=M'], then substituting [x:=N] to both
+sides should preserve the equality.
+*)
 Proposition subst_apply_rand :
   forall (M M' N:Term) (x:Id),
   M=M' -> [x:=N]M = [x:=N]M'.
@@ -228,7 +266,10 @@ Proof.
   intros. rewrite H. reflexivity.
 Qed.
 
-(** Barendregt 2.1.17.ii *)
+(**
+(Barendregt 2.1.17.ii) If we have [N=N'], then substituting [x:=N]
+should produce the same results as substituting [x:=N'].
+*)
 Proposition subst_apply_rator :
   forall (M N N':Term) (x:Id),
   N=N' -> [x:=N]M = [x:=N']M.
@@ -236,7 +277,10 @@ Proof.
   intros. rewrite H. reflexivity.
 Qed.
 
-(** Barendregt 2.1.17.iii *)
+(**
+(Barendregt 2.1.17.iii) The most general situation, when we have [M=M'],
+and [N=N'], then substituting [[x:=N] M] should be equal to [[x:=N']M'].
+*)
 Proposition subst_apply_rand_rator :
   forall (M M' N N':Term) (x:Id),
   M=M' -> N=N' -> [x:=N]M = [x:=N']M'.
@@ -244,7 +288,4 @@ Proof.
   intros.
   rewrite H. rewrite H0. reflexivity.
 Qed.
-
 End Substitute.
-End Untyped.
-End src.
