src/Untyped/TractLib.v
@@ -1,0 +1,92 @@
+Module Export TractLib.
+Require Import List.
+Require Import String.
+Require String. Open Scope string_scope.
+
+(**
+A lot of this is borrowed from Pierce, et al.'s, _Software Foundations_
+library, which is -- in turn -- borrowed from elsewhere.
+*)
+
+Definition relation (X:Type) := X -> X -> Prop.
+
+Definition deterministic {X: Type} (R: relation X) :=
+  forall x y1 y2 : X, R x y1 -> R x y2 -> y1 = y2. 
+
+Inductive multi (X:Type) (R: relation X) 
+                            : X -> X -> Prop :=
+  | multi_refl  : forall (x : X),
+                 multi X R x x
+  | multi_step : forall (x y z : X),
+                    R x y ->
+                    multi X R y z ->
+                    multi X R x z.
+Implicit Arguments multi [[X]]. 
+
+Ltac move_to_top x :=
+  match reverse goal with
+  | H : _ |- _ => try move x after H
+  end.
+
+Tactic Notation "assert_eq" ident(x) constr(v) :=
+  let H := fresh in
+  assert (x = v) as H by reflexivity;
+  clear H.
+
+Tactic Notation "Case_aux" ident(x) constr(name) :=
+  first [
+    set (x := name); move_to_top x
+  | assert_eq x name; move_to_top x
+  | fail 1 "because we are working on a different case" ].
+
+Tactic Notation "Case" constr(name) := Case_aux Case name.
+Tactic Notation "SCase" constr(name) := Case_aux SCase name.
+Tactic Notation "SSCase" constr(name) := Case_aux SSCase name.
+Tactic Notation "SSSCase" constr(name) := Case_aux SSSCase name.
+Tactic Notation "SSSSCase" constr(name) := Case_aux SSSSCase name.
+Tactic Notation "SSSSSCase" constr(name) := Case_aux SSSSSCase name.
+Tactic Notation "SSSSSSCase" constr(name) := Case_aux SSSSSSCase name.
+Tactic Notation "SSSSSSSCase" constr(name) := Case_aux SSSSSSSCase name.
+
+Tactic Notation "multi_cases" tactic(first) ident(c) :=
+  first;
+  [ Case_aux c "multi_refl" | Case_aux c "multi_step" ].
+
+
+Theorem multi_R : forall (X:Type) (R:relation X) (x y : X),
+  R x y -> multi R x y.
+Proof.
+  intros X R x y r.
+  apply multi_step with y. apply r. apply multi_refl.
+Qed.
+
+Theorem multi_trans :
+  forall (X:Type) (R: relation X) (x y z : X),
+      multi R x y ->
+      multi R y z ->
+      multi R x z.
+Proof.
+  intros X R x y z G H.
+  multi_cases (induction G) Case.
+    Case "multi_refl". assumption.
+    Case "multi_step".
+      apply multi_step with y. assumption.
+      apply IHG. assumption.
+Qed.
+
+(** Helper lemmas, which should be refactored into a different module.
+
+Principle of explosion: from a contradiction, we can prove anything. 
+*)
+Theorem ex_falso_quodlibet : forall (P:Prop),
+  False -> P.
+Proof.
+  intros P contra.
+  inversion contra.
+Qed.
+
+Lemma list_membership :
+  forall (A:Type) (x:A) (l1 l2:list A),
+  (In x l1)\/(In x l2) <-> In x (l1 ++ l2).
+Proof. intuition. Qed.
+End TractLib.
